Logic/Modal/Kripke/Semantics.lean
@@ -31,7 +31,7 @@ lemma dia_def : x ⊧ ◇p ↔ ∃ y, x ≺ y ∧ y ⊧ p := by simp [Kripke.Sat
 
 lemma not_def : x ⊧ ~p ↔ ¬(x ⊧ p) := by
   induction p using Formula.rec' generalizing x with
-  | _ => simp_all [Satisfies]; try tauto;
+  | _ => simp_all [Satisfies];
 instance : Semantics.Not (M.World) := ⟨not_def⟩
 
 lemma imp_def : x ⊧ p ⟶ q ↔ (x ⊧ p) → (x ⊧ q) := by tauto;
