Logic/Modal/PLoN/Semantics.lean
@@ -69,7 +69,7 @@ lemma box_def : x ⊧ □p ↔ ∀ y, x ≺[p] y → y ⊧ p := by simp [PLoN.Sa
 
 lemma not_def : x ⊧ ~p ↔ ¬(x ⊧ p) := by
   induction p using Formula.rec' generalizing x with
-  | _ => simp_all [Satisfies]; try tauto;
+  | _ => simp_all [Satisfies];
 instance : Semantics.Not (M.World) := ⟨not_def⟩
 
 lemma imp_def : x ⊧ p ⟶ q ↔ (x ⊧ p) → (x ⊧ q) := by tauto;
